src/Refine.v
@@ -1,6 +1,7 @@
 Require Import
   Coq.Program.Program
   Coq.Program.Tactics
+  Coq.omega.Omega
   Coq.Lists.List.
 
 Require Export
@@ -12,20 +13,130 @@ Import ListNotations.
 
 Generalizable All Variables.
 
-Inductive relate {a} : forall {effs}, Eff effs a -> a -> Prop :=
-  | RelatePure : forall effs v, relate (effs:=effs) (Pure v) v
+Fixpoint InT `(a : A) (l : list A) : Type :=
+  match l with
+  | [] => False
+  | b :: m => (b = a) + InT a m
+  end.
 
-  | RelateImpureThis :
-      forall `{Computes eff} effs v
-             x u (k : x -> Eff (eff :: effs) a),
-        forall i, computes u i -> relate (k i) v ->
-        relate (Impure (UThis u) k) v
+Program Instance Union_Computes {s} :
+  (forall eff, InT eff effs -> Computes s eff) -> Computes s (Union effs) := {
+  computes := fun _ u v => _
+}.
+Next Obligation.
+  induction effs; intros.
+    now inversion v.
+  inversion v; subst; clear v.
+    refine (computes u X1 X X0).
+    apply H.
+    now left.
+  apply IHeffs; auto.
+  intros.
+  apply H.
+  now right.
+Defined.
 
-  | RelateImpureThat :
-      forall eff effs v
-             x u (k : x -> Eff (eff :: effs) a) ret bind,
-        relate (Impure u (fun x => handleRelay ret bind (k x))) v ->
-        relate (Impure (UThat u) k) v.
+Section Relate.
 
-Definition refine {effs a} (old new : Eff effs a) : Prop :=
-  forall v, relate old v -> relate new v.
+Variable s : Type.
+Variable effs : list (Type -> Type).
+Variable a : Type.
+
+Hypothesis Hcomputes : forall eff, InT eff effs -> Computes s eff.
+
+Inductive relate : s -> Eff effs a -> s -> a -> Prop :=
+  | RelatePure :
+      forall st v, relate st (Pure v) st v
+
+  | RelateImpure :
+      forall st st' st'' v x u (k : x -> Eff effs a),
+        forall i, computes st u st' i ->
+        relate st' (k i) st'' v ->
+        relate st (Impure u k) st'' v.
+
+Definition refine (st : s) (old new : Eff effs a) : Prop :=
+  forall (st' : s) v, relate st old st' v -> relate st new st' v.
+
+Require Import
+  Hask.Control.Monad
+  RWS.
+
+End Relate.
+
+Program Instance Choice_Computes {s} : Computes s Choice := {
+  computes := fun _ st '(Pick P) st' v => P v /\ st = st'
+}.
+
+Program Instance State_Computes {s} : Computes s (State s) := {
+  computes := fun _ st a st' v => State_func a st = (st', v)
+}.
+
+Lemma choice_and_state_computes :
+  forall eff : Type -> Type,
+    InT eff [Choice; State (nat : Type)] -> Computes nat eff.
+Proof.
+  intros.
+  destruct X; subst.
+    apply Choice_Computes.
+  destruct i; subst.
+    apply State_Computes.
+  inversion i.
+Defined.
+
+Example relate_ex :
+  relate _ _ _ choice_and_state_computes
+    0
+    (send (Put 10) ;;
+     x <- send Get ;
+     y <- send (Pick (fun x => x <= 10));
+     pure (x + y))
+    10
+    15.
+Proof.
+  simpl.
+  repeat (eapply RelateImpure; eauto; try reflexivity).
+    instantiate (1 := 5).       (* here the Pick is resolved *)
+    simpl.
+    unfold eq_rect_r, eq_rect, eq_sym; simpl.
+    split.
+      omega.
+    reflexivity.
+  constructor.
+Qed.
+
+Example refine_works :
+  refine _ _ _ choice_and_state_computes
+    10
+    (send (Put 10) ;;
+     x <- send Get ;
+     y <- send (Pick (fun x => x <= 10));
+     pure (x + y))
+    (y <- send (Pick (fun x => x <= 30)); (* wrong! *)
+     pure y).
+Proof.
+  simpl.
+  repeat intro.
+  inversion H; subst; clear H.
+  apply inj_pair2 in H4; subst.
+  apply inj_pair2 in H1; subst.
+  inversion H6; subst; clear H6.
+  inversion H7; subst; clear H7.
+  apply inj_pair2 in H0; subst.
+  apply inj_pair2 in H3; subst.
+  inversion H5; subst; clear H5.
+  inversion H6; subst; clear H6.
+  apply inj_pair2 in H0; subst.
+  apply inj_pair2 in H3; subst.
+  inversion H5; subst; clear H5.
+  inversion H7; subst; clear H7.
+  econstructor.
+    simpl.
+    unfold eq_rect_r, eq_rect, eq_sym; simpl.
+    split.
+      instantiate (1 := i + 10).
+      omega.
+    reflexivity.
+  replace (S (S (S (S (S (S (S (S (S (S i))))))))))
+     with (i + 10) by omega.
+  constructor.
+Qed.                            (* this was not a refinement! *)
